???????????

HOL_To_IMP_Minus/Refinements/HOL_To_IMP_Minus_Datatypes.thy
@@ -1,64 +1,160 @@
 \<^marker>\<open>creator "Kevin Kappelmann"\<close>
 theory HOL_To_IMP_Minus_Datatypes
   imports
-    HOL_To_HOL_Nat.HOL_To_HOL_Nat_Basics
-    HOL_To_IMP_Minus_Primitives
+    HOL_To_IMP_Minus_Arithmetics
+  keywords
+    "unrelate_nat" :: thy_decl
 begin
+
+(* obviously don't do this, but how to declare constants from within a command??? *)
+consts some_const :: "nat \<Rightarrow> nat \<Rightarrow> nat"
 
 locale HOL_To_HOL_Nat =
   notes transport_eq_id.partial_equivalence_rel_equivalenceI[per_intro del]
   and transport_eq_restrict_id.partial_equivalence_rel_equivalence[per_intro del]
 begin
 
-case_of_simps append_eq_case : append.simps
-function_compile_nat append_eq_case
+fun rev_aux :: "'a list \<Rightarrow> 'a list \<Rightarrow> 'a list" where
+  "rev_aux acc [] = acc" |
+  "rev_aux acc (x # xs) = rev_aux (x # acc) xs"
 
-case_of_simps rev_eq_case : rev.simps
-function_compile_nat rev_eq_case
+case_of_simps rev_aux_eq (* [simplified Nitpick.case_nat_unfold] *) : rev_aux.simps
+
+function_compile_nat rev_aux_eq
+print_theorems
+
+(*
+thm zip.simps
+
+fun zip :: "'a list \<Rightarrow> 'b list \<Rightarrow> ('a \<times> 'b) list" where
+  "zip (x # xs) (y # ys) = (x, y) # zip xs ys" |
+  "zip _ _ = []"
+
+case_of_simps zip_eq : zip.simps
+function_compile_nat zip_eq
+print_theorems
+thm zip_nat_eq_unfolded[simplified case_list_nat_def]
+fun zip_nat_magic :: "nat \<Rightarrow> nat \<Rightarrow> nat"  where
+  "zip_nat_magic x xa =
+  (if fst_nat x = 0 then Nil_nat
+   else if fst_nat xa = 0 then Nil_nat
+   else
+     Cons_nat
+       (Pair_nat (fst_nat (snd_nat x)) (fst_nat (snd_nat xa)))
+       (zip_nat_magic (snd_nat (snd_nat x)) (snd_nat (snd_nat xa))))"
+*)
+
+definition rev :: "'a list \<Rightarrow> 'a list" where
+  "rev = rev_aux []"
+
+function_compile_nat rev_def
 
 end
+
+
 context HOL_To_IMP_Minus
 begin
 
-(*dummy stubs; need to compile fst_nat, snd_nat, pair_nat*)
-(*then we could compile constructors and automatically generated functions:*)
-thm Cons_nat_def
+compile_nat Cons_nat_def
+HOL_To_IMP_Minus_correct Cons_nat by cook
 
-declare_compiled_const fst_nat
-  return_register "fst.ret"
-  argument_registers "fst.args.x"
-  compiled suc_IMP
+compile_nat Nil_nat_def
+HOL_To_IMP_Minus_correct Nil_nat by cook
 
-declare_compiled_const snd_nat
-  return_register "fst.ret"
-  argument_registers "fst.args.x"
-  compiled suc_IMP
 
-declare_compiled_const Cons_nat
-  return_register "fst.ret"
-  argument_registers "fst.args.x" "fst.args.y"
-  compiled suc_IMP
+ML\<open>
 
-declare_compiled_const Pure.type
-  return_register "fst.ret"
-  argument_registers
-  compiled suc_IMP
+(* structure BU = BNF_Util *)
+structure HTHNU = HOL_To_HOL_Nat_Util
 
-context
-  fixes xs' ys' :: "('a :: compile_nat) list"
-  assumes rels: "Rel_nat xs xs'" "Rel_nat xs ys'"
-begin
+(*
+fun register_fun binding_name lhs rhs lthy =
+  let
+    val l = Syntax.pretty_term lthy #> Pretty.writeln
+    val _ = (@{print} (binding_name, lhs, rhs); l lhs; l rhs)
+    val fixes = [(binding_name, SOME (Term.head_of lhs |> Term.fastype_of), NoSyn)]
+    val specs = [((Binding.empty_atts, BU.mk_Trueprop_eq (lhs, rhs)), [], [])]
+  in Function_Fun.add_fun fixes specs Function_Fun.fun_config lthy end *)
 
-lemmas test = HOL_To_HOL_Nat.append_nat_eq_unfolded[OF rels, unfolded case_list_nat_def]
-definition "blub x y \<equiv> HOL_To_HOL_Nat.append_nat TYPE('a) x y"
+fun unrelate_nat_command f_eq _ lthy =
+  let
+    val (lhs, rhs) = HTHNU.dest_eq_equals_thm f_eq
+    val f as (f_name, f_typ) =  lhs |> Term.head_of |> Term.dest_Const
 
-lemma blub_rec: "blub x y =
-  (if fst_nat x = 0 then y else Cons_nat (fst_nat (snd_nat x)) (blub (snd_nat (snd_nat x)) y))"
-  unfolding blub_def by (subst test) (rule refl)
+    fun is_typrep (Type (@{type_name itself}, [_])) = true | is_typrep _ = false
+    fun is_nat (Type (@{type_name nat}, [])) = true | is_nat _ = false
+    val (typrep_arg_count, rem_args) =
+      Term.args_of lhs
+      |> chop_prefix (is_typrep o Term.fastype_of)
+      |>> List.length
+    val _ =
+      (List.all (is_nat o Term.fastype_of) rem_args andalso is_nat (Term.fastype_of lhs))
+      orelse raise TERM ("Expected type: function taking zero or more '_ itself' arguments, followed by zero or more 'nat' arguments, and returning 'nat'", [lhs])
 
-compile_nat blub_rec
+    val f'_typ = List.map Term.fastype_of rem_args ---> @{typ nat}
 
+    (* val _ = Proof_Context.theory_of *)
+    (* val _ = Proof_Context.init_global *)
+    val t = @{const some_const}
+    val binding = Binding.name (Term.dest_Const_name t) (* "some_const" *)
+    (* val (t, lthy' : theory) =
+      Sign.declare_const lthy ((binding, f'_typ), NoSyn) (Context.theory_of (Context.Proof lthy)) *)
+
+    val f'_name = Term.dest_Const_name t
+    val _ = @{print} f'_name
+    val f' = Const (f'_name, f'_typ)
+
+    val rewrite_vars = Term.map_aterms (fn Var ((name, _), typ) => Free (name, typ) | t => t)
+
+    fun rewrite_rhs t =
+      let
+        val (head, args) = Term.strip_comb t
+        val is_rec_call = case head of Const g => f = g | _ => false
+        val _ = (is_rec_call andalso length args < typrep_arg_count)
+          andalso raise TERM ("Can't strip all '_ itself' arguments", [t])
+        val head' = if is_rec_call then f' else head
+        val args' =
+          (if is_rec_call then drop typrep_arg_count args else args)
+          |> map rewrite_rhs
+      in Term.list_comb (head', args') end
+
+    val lhs' = Term.list_comb (f', rem_args) |> rewrite_vars
+    val rhs' = rhs |> rewrite_rhs |> rewrite_vars
+
+    (* val _ = HOLogic.mk_eq (lhs', rhs') |> Thm.cterm_of lthy |> @{print} *)
+
+    val lthy' = HTHNU.register_fun binding lhs' rhs' lthy
+
+  in lthy' end
+
+local
+  val parser = Parse.thm -- Scan.option (\<^keyword>\<open>basename\<close> |-- Parse.name_position)
+in
+  val _ = Outer_Syntax.local_theory
+    \<^command_keyword>\<open>unrelate_nat\<close>
+    "remove Rel_nat/rel_fun assumptions and TYPE(_) args"
+    (parser >> (fn ((thm_ref, _), namepos_opt) => fn lthy =>
+      let val thm = Proof_Context.get_fact lthy thm_ref |> the_single
+      in unrelate_nat_command thm namepos_opt lthy end))
 end
+\<close>
+
+lemmas rev_aux_nat_eq = HOL_To_HOL_Nat.rev_aux_nat_eq_unfolded[simplified case_list_nat_def]
+unrelate_nat rev_aux_nat_eq basename base1
+
+
+(* TODO: magic, goal: *)
+(*
+fun rev_aux_nat_magic where
+  "rev_aux_nat_magic x xa =
+    (if fst_nat xa = 0 then x
+     else rev_aux_nat_magic (Cons_nat (fst_nat (snd_nat xa)) x) (snd_nat (snd_nat xa)))"
+
+declare rev_aux_nat_magic.simps[simp del]
+
+compile_nat rev_aux_nat_magic.simps
+HOL_To_IMP_Minus_correct rev_aux_nat_magic by (cook mode = tailcall)
+*)
 
 end
 
